Terminada Lex y is_lex

checker.v
@@ -1,5 +1,6 @@
 Require Import Vectors.Vector.
 Require Import ZArith.
+Require Import Lia.
 
 (*We import the definions and functions we defined for the constraints*)
 Require Import constraint.
@@ -28,7 +29,6 @@ Definition imp_checker_snd {n_v : nat} {n_c : nat } (chkr : @imp_checker (S n_v)
   forall (cs : constraints) (c : constraint),
     chkr cs c = true ->
      cs_imp_c cs c.
-
 
 Lemma comb_conic_is_model : forall {n_v n_c : nat},
   forall (cs : constraints) (c_comb : @constraint (S n_v)) (d : t nat n_c) (model : assignment),
@@ -91,15 +91,15 @@ Proof.
 Qed.
 
 Theorem farkas : forall {n_v n_c : nat},
-  forall (cs : constraints) (d : t nat n_c) (c_comb c : @constraint (S n_v)),
+  forall (cs : constraints) (d : t nat n_c) (c_comb : @constraint (S n_v)),
     is_equal d cs c_comb = true ->
-    forall (model : @assignment n_v), 
+    forall (model : @assignment n_v) (c : @constraint (S n_v)), 
     is_model cs (adapt model) = true ->
     is_gt_on_last c_comb c = true ->
     is_model_c c (adapt model) = true.
 Proof.
-  intros n_v n_c cs d c_comb c.
-  intros h0 model h1 h2.
+  intros n_v n_c cs d c_comb.
+  intros h0 model c h1 h2.
   apply (@comb_conic_is_model n_v n_c cs c_comb d model) in h0.
   apply (@farkas_gt n_v c_comb c model) in h0.
   assumption. assumption. assumption.
@@ -128,7 +128,6 @@ Qed.
 
 Definition lex_function {n_var : nat} := t Z (S n_var).
 
-
 (*This function receives a lex funciton and returns the corresponding constraint*)
 Definition c_of_f {n_var : nat} (f : @lex_function n_var) :  @constraint (S (n_var + n_var)) :=
   let rev_f := (rev f) in
@@ -151,22 +150,12 @@ Definition cs_f_i_minus_f_i' {n_var : nat} (f : @lex_function n_var) : @constrai
 Definition cs_f_i'_minus_f_i {n_var : nat} (f : @lex_function n_var) : @constraint (S (n_var + n_var)) :=
   vect_mul_Z (-1) (cs_f_i_minus_f_i' f).
 
+Definition cs_of_two {n_var : nat} (c c' : @constraint n_var) : constraints :=
+  shiftin c' (shiftin c []).
 
 (* This function receive a couple of contraint and returns its composition in a constraints*)
 Definition new_cs {n_var n_c : nat} (cs : @constraints (S (n_var + n_var)) n_c)  (f : @lex_function n_var) : constraints :=
  shiftin (cs_f_i_minus_f_i' f) (shiftin (cs_f_i'_minus_f_i f) cs).
-
-(*
-
-    list_f = f1::fs ->
-     cs => f1>=0 ->
-      cs =>f1-f1'>=0 ->
-       (Lex f1-f1'<=0::-f1+f1'<=0::cs fs) -> Lex cs list_f
-*)
-
-Definition cs_of_two {n_var : nat} (c c' : @constraint n_var) : constraints :=
-  shiftin c' (shiftin c []).
-
 
 Definition cs_f_i_minus_f_i'_is_zero {n_var : nat} (f : @lex_function n_var) :  constraints :=
   cs_of_two (cs_f_i_minus_f_i' f) (cs_f_i'_minus_f_i f).
@@ -177,35 +166,64 @@ Require Import List.
 
 Import ListNotations.
 
+Fixpoint my_of_list (n : nat) (l: list nat) : option (t nat n) :=
+  match l with
+  | []%list =>
+      match n with
+      | O => Some (const 0%nat 0)
+      | _ => None
+      end
+  | (x::xs)%list =>
+      match n with
+      | O => None
+      | S n' => match my_of_list n' xs with
+                | None => None
+                | Some v => Some (x::v)%vector
+                end
+      end
+  end.
+
+Definition lex_func {n_var n_c} (cs : @constraints (S n_var) n_c) (d : t nat n_c) (f : @constraint (S n_var)) : bool :=
+  is_gt_on_last (comb_conic d cs) f.
+                                                                                      
 Fixpoint is_lex {n_var n_c : nat} (cs : @constraints (S (n_var + n_var)) n_c) (list_f : list (@lex_function n_var)) (list_of_d : list ((list_d)*(list_d))) : bool :=
   match list_f with
   | [] => match list_of_d with
           | [] => false
           | d::ds => let d_i := fst d in
-                     let vec_d := of_list d_i in
-                     if (length d_i =? n_c)%nat then is_minus_one (comb_conic vec_d cs)
-                     else false
+                     let vec_d := my_of_list n_c d_i in
+                     match vec_d with
+                     | None => false
+                     | Some v => is_minus_one (comb_conic v cs)
+                     end
           end
   | f::fs =>let f_i := c_of_f f in
             let f_i_minus_f_i' := cs_f_i_minus_f_i' f in
             match list_of_d with
             | [] => false
-            | d::ds => ((is_equal (fst d) cs f_i) &&
-                          (is_equal (snd d) cs f_i_minus_f_i') &&
-                          (is_lex (new_cs cs f) fs ds)
-                       )%bool
+            | d::ds =>
+                let d_i_1 := fst d in
+                let d_i_2 := snd d in
+                let vec_d_1 := my_of_list n_c d_i_1 in
+                let vec_d_2 := my_of_list n_c d_i_2 in
+                match vec_d_1 with
+                | None => false
+                | Some v1 => match vec_d_2 with
+                             | None => false
+                             | Some v2 => ((lex_func cs v1 f_i) &&
+                                             (lex_func cs v2 f_i_minus_f_i') &&
+                                             (is_lex (new_cs cs f) fs ds)
+                                          )%bool
+                             end
+                end
             end
   end.
- 
-
-
 
 (*Inductive proposition on the lex functions*)
 Inductive Lex {n_var n_c : nat} : (@constraints (S (n_var + n_var)) n_c) -> list (@lex_function n_var) -> Prop :=
 | basic
     (cs : (@constraints (S (n_var + n_var)) n_c))
     (list_f : list (@lex_function n_var))
-    (H : (length list_f) = 0%nat)
     (H1 : unsat cs)
   : (Lex cs list_f)    
 | other
@@ -213,11 +231,72 @@ Inductive Lex {n_var n_c : nat} : (@constraints (S (n_var + n_var)) n_c) -> list
     (list_f : list (@lex_function n_var))
     (f : @lex_function n_var)
     (fs : list (@lex_function n_var))
-    (Hl : (length list_f) = S (length fs))
     (H' : list_f = f::fs)
-    (H1 : Lex  (new_cs cs f) fs)
-    (H2 : cs_imp_cs' cs (cs_f_i_minus_f_i'_is_zero f))
+    (H1 : cs_imp_c cs (cs_f_i_minus_f_i' f))
+    (H2 : cs_imp_c cs (c_of_f f))
+    (H3 : Lex  (new_cs cs f) fs)
   : (Lex cs list_f).
-                                                 
-                                                   
 
+Lemma aux_eq_comb_conic :
+  forall {n_var n_c : nat}
+         (cs : @constraints (S n_var) n_c)
+         (d : t nat n_c),
+    is_equal d cs (comb_conic d cs) = true.
+Proof.
+  intros n_var n_c cs d.
+  unfold is_equal.
+  rewrite eqb_eq.
+  reflexivity.
+  exact eq_snd.
+Qed. 
+  
+Lemma is_equal_imp :
+  forall {n_var n_c : nat}
+         (cs : @constraints (S n_var) n_c)
+         (f : @constraint (S n_var))
+         (d : t nat n_c),
+    lex_func cs d f = true -> cs_imp_c cs f.
+Proof.
+  intros n_var n_c cs f d.
+  intro H.
+  unfold lex_func in H.  
+  unfold cs_imp_c.
+  intros model H1. Check farkas.
+  apply (@farkas n_var n_c cs d (comb_conic d cs) (@aux_eq_comb_conic n_var n_c cs d) model f) in H1.
+  exact H1.
+  exact H.
+Qed.
+
+Theorem is_lex_imp_Lex :
+  forall {n_var : nat}
+         (list_f : list (@lex_function n_var))
+         {n_c : nat}
+         (cs : @constraints (S (n_var + n_var)) n_c)
+         (list_of_d : list ((list_d)*(list_d))),
+    is_lex cs list_f list_of_d = true -> Lex cs list_f.
+Proof.
+  intros n_var list_f.
+  induction list_f as [| f1 fs IHf'].
+  - simpl. intros n_c cs list_of_d.
+    induction list_of_d as [| d1 ds IHd'].
+    -- intro H. apply Bool.diff_false_true in H.
+       contradiction.
+    -- destruct (my_of_list n_c (fst d1)).
+       --- intro H. apply unsat_suf in H. exact (basic cs [] H).
+       --- intro H. apply Bool.diff_false_true in H.
+           contradiction.
+  - simpl. intros n_c cs list_of_d H.
+    induction list_of_d as [| d1 ds IHd'].
+    --  apply Bool.diff_false_true in H.
+       contradiction.
+    -- destruct (my_of_list n_c (fst d1)).
+       destruct (my_of_list n_c (snd d1)).
+       --- apply andb_prop in H. destruct H. apply andb_prop in H. destruct H.
+           apply is_equal_imp in H. apply is_equal_imp in H1.
+           apply (@other n_var n_c cs (f1::fs) f1 fs (eq_refl) H1 H).
+           apply (@IHf' (S (S (n_c))) (new_cs cs f1) ds H0).
+       --- apply Bool.diff_false_true in H.
+           contradiction.
+       --- apply Bool.diff_false_true in H.
+           contradiction.
+Qed.         
